Added some extra functions:
"GET" (gets the nth character of a string - overloaded to prime),
"TRANSFORM" (apply a list function to a string),
"isUpper", "isHexDigit" etc. (tests on character classes).

Also enabled case splitting on character code
e.g. ``c`` goes to ``CHR n`` for n < 256.

src/string/stringSyntax.sig
@@ -52,6 +52,7 @@ sig
   val fromMLstring      : string -> term
   val fromHOLstring     : term -> string
 
+  val is_char_literal   : term -> bool
   val is_string_literal : term -> bool
    
   val lift_char         : hol_type -> char -> term
